high/Veritas.Interleave.fsti
@@ -149,6 +149,19 @@ let telem (#a:eqtype) (il:interleaving a {length il > 0}): a =
 val prefix_identity (#a:eqtype) (il:interleaving a)
   : Lemma (ensures prefix il (length il) == il)
 
+val prefix_int_add (#a:eqtype) (i:interleaving a { IntAdd? (IL?.prf i) }) (n:nat{n <= length i})
+  : Lemma 
+    (let IL _ _ (IntAdd _ _ prf) = i in
+     prefix i n == 
+     IL _ _ (IntAdd _ _ (IL?.prf (prefix (IL _ _ prf) n))))
+  
+val prefix_int_extend (#a:eqtype) (i:interleaving a { IntExtend? (IL?.prf i) }) (n:nat{n <= length i})
+  : Lemma
+    (let IL _ _ (IntExtend s ss prf x j) = i in
+     (if n <= Seq.length s
+      then prefix i n == prefix (IL s ss prf) n
+      else prefix i n == i))
+
 val hprefix_extend (#a:eqtype) (s:seq a) (ss:sseq a)
                     (il:interleave s ss)
                     (x:a)
